src/LamRefLogicFactsTotal.v
@@ -62,22 +62,22 @@ Theorem triple_weaken (V : Set) (e : Expr V) P P' Q Q' :
   hoare_triple e P Q ->
   hoare_triple e P' Q'.
 Proof.
-  unfold hoare_triple, sa_implies. eauto.
-Qed.
-
-Theorem triple_value' (V : Set) (v : Value V) (P : StateAssertion V) :
-  hoare_triple v P (fun _ c => <[c = 0]> <*> P).
-Proof.
-  unfold hoare_triple, sa_star, sa_pure, sa_empty, disjoint_maps.
-  intros v' c m m' Hred. inversion_cost_red.
-  intro p. repeat eexists; eauto.
+  unfold hoare_triple, sa_implies. intros ? ? H ? ?.
+  edestruct H as [? [? [? [? ?]]]]; eauto 10.
 Qed.
 
 Theorem triple_value (V : Set) (v : Value V) :
-  hoare_triple v <[]> (fun _ c => <[c = 0]>).
+  hoare_triple v <[]> (fun v' c => <[v' = v /\ c = 0]>).
 Proof.
   unfold hoare_triple, sa_pure, sa_empty.
-  intros v' c m m' Hred. inversion_cost_red. auto.
+  intros m Hm. subst. eauto 10 with lamref.
+Qed.
+
+Theorem triple_value' (V : Set) (v : Value V) (P : StateAssertion V) :
+  hoare_triple v P (fun v' c => <[v' = v /\ c = 0]> <*> P).
+Proof.
+  unfold hoare_triple, sa_star, sa_pure, sa_empty, disjoint_maps.
+  eauto 15 with lamref.
 Qed.
 
 Theorem triple_value_untimed (V : Set) (v : Value V) (P : StateAssertion V) :
@@ -93,8 +93,8 @@ Theorem triple_lam (V : Set) (e : Expr _) (v : Value V) P Q :
   hoare_triple (subst_e e v) P (fun v c => Q v (1+c)) ->
   hoare_triple ((-\e) <* v) P Q.
 Proof.
-  unfold hoare_triple. intros Hhoare v' c m m' Hred. inversion_cost_red.
-  eapply Hhoare. inversion_red. auto.
+  unfold hoare_triple. intros.
+  edestruct H as [? [? [? [? ?]]]]; eauto 10 with lamref.
 Qed.
 
 (*Theorem triple_seq (V : Set) (e1 e2 : Expr V) P1 P2 Q1 Q2 :
@@ -108,24 +108,34 @@ Proof.
   intros.
   inversion_cost_red. inversion_red.
 *)
+
+Theorem triple_app (V : Set) (e1 e2 : Expr V) e1' (v2 : Value V)
+  P1 P2 P3 Q3 c1 c2 :
+  hoare_triple e1 P1 (fun v c => <[v = (-\e1') /\ c = c1]> <*> P2) ->
+  hoare_triple e2 P2 (fun v c => <[v = v2 /\ c = c2]> <*> P3) ->
+  hoare_triple (subst_e e1' v2) P3 (fun v c => Q3 v (c1 + c2 + 1 + c)) ->
+  hoare_triple (App e1 e2) P1 Q3.
+Proof.
+  unfold hoare_triple, sa_exists, sa_star, sa_single, sa_pure, sa_empty,
+    sa_implies, disjoint_maps, labels.
+  intros.
+  edestruct H as [? [? [? [? [? [? [[[? ?] ?] [? [? ?]]]]]]]]]; eauto. subst.
+  edestruct H0 as [? [? [? [? [? [? [[[? ?] ?] [? [? ?]]]]]]]]]; eauto. subst.
+  edestruct H1 as [? [? [? [? ?]]]]; eauto 10 using big_red_app.
+Qed.
+
 Theorem triple_bneg (V : Set) (e : Expr V) (b : bool) P Q :
-  P ->> Is_Valid_Map ->
   hoare_triple e P (fun v c => <[v = Bool b]> <*> Q (1+c)) ->
   hoare_triple ([~] e)
     P
     (fun v c => <[v = Bool (negb b)]> <*> Q c).
 Proof.
-  unfold Is_Valid_Map, labels. find_red_cases.
-  - edestruct H0 as [? [? [[? ?] [? [? ?]]]]]; eauto with lamref. subst.
-    simpl in *. injection H1 as [].
-    inversion_cost_red. repeat eexists; eauto.
-  - edestruct cost_red_split1_exists; [|apply red_unop| |].
-    + eauto with lamref.
-    + eauto.
-    + econstructor. eauto with lamref. eauto.
-    +
-    
-Admitted.
+  unfold hoare_triple, sa_exists, sa_star, sa_single, sa_pure, sa_empty,
+    disjoint_maps, labels.
+  intros.
+  edestruct H as [? [? [? [? [? [? [[? ?] [? [? ?]]]]]]]]]; eauto.
+  subst. eauto 15 using big_red_bneg.
+Qed.
 
 Theorem triple_ineg (V : Set) (i : Z) :
   @hoare_triple V ([--] Int i)
